SSA/Projects/CIRCT/Handshake-to-DC/ForkToken.lean
@@ -1,4 +1,4 @@
-import SSA.Projects.CIRCT.DCxComb.DCxComb
+import SSA.Projects.CIRCT.DCxComb.DCxCombFunctor
 import SSA.Projects.CIRCT.Handshake.Handshake
 import SSA.Projects.CIRCT.Stream.Stream
 import SSA.Projects.CIRCT.Stream.WeakBisim
@@ -33,13 +33,18 @@ def forkToken := [DCxComb_com| {
 #print axioms forkToken
 
 def ofList (vals : List (Option α)) : Stream α :=
-  fun i => (vals.get? i).join
+  fun i => vals[i]?.join
 
-def x : DCxCombOp.TokenStream := ofList [some (), none, some (), some (), none]
+def x : DCOp.TokenStream := ofList [some (), none, some (), some (), none]
 
-def test : DCxCombOp.TokenStream × DCxCombOp.TokenStream :=
+def test : DCOp.TokenStream × DCOp.TokenStream :=
   forkToken.denote (Ctxt.Valuation.ofHVector (.cons x <| .nil))
 
 open Ctxt in
-theorem equiv_forkToken (streamT : DCxCombOp.TokenStream) :
-  (HandshakeOp.fork streamT).fst ~ (forkToken.denote (Valuation.ofHVector (.cons streamT <| .nil))).fst := by sorry
+theorem equiv_forkToken (streamT : DCOp.TokenStream) :
+    (HandshakeOp.fork streamT).fst ~ (forkToken.denote (Valuation.ofHVector (.cons streamT <| .nil))).fst := by
+  simp only [forkToken, get?.eq_1, Var.zero_eq_last, Valuation.ofHVector, Ctxt.ofList.eq_1,
+    Com.denote_var, EffectKind.toMonad_pure, Com.denote_ret, Valuation.snoc_last, Id.pure_eq,
+    Id.bind_eq]
+  simp [HandshakeOp.fork, MLIR2DC.Op.fork]
+  sorry
