SSA/Projects/CIRCT/Handshake-to-DC/ForkData.lean
@@ -1,5 +1,5 @@
 import SSA.Projects.CIRCT.Handshake.Handshake
-import SSA.Projects.CIRCT.DCxComb.DCxComb
+import SSA.Projects.CIRCT.DCxComb.DCxCombFunctor
 import SSA.Projects.CIRCT.Stream.Stream
 import SSA.Projects.CIRCT.Stream.WeakBisim
 import SSA.Core.Tactic
@@ -12,7 +12,7 @@ import SSA.Core.Util
 namespace CIRCTStream
 namespace Stream.Bisim
 
-theorem corec₂_eq_tok (x : DCxCombOp.TokenStream):
+theorem corec₂_eq_tok (x : DCOp.TokenStream):
   (corec₂ x fun x => Id.run (x 0, x 0, tail x)) = (corec₂ x fun x => Id.run (x 0, x 0, x.tail)) := by
   apply corec₂_eq_corec₂_of
   rotate_left 2
@@ -37,18 +37,18 @@ theorem EqIsBisim {α} : @IsBisim α Eq := by
   intros a; exists 0; exists 0
   and_intros; all_goals first | rfl | intros _ h; cases h
 
-theorem fork_hs_dc_equiv_fst (x : DCxCombOp.TokenStream):
-    (DCxCombOp.fork (x)).fst ~ (HandshakeOp.fork (x)).fst := by
-  simp [Bisim, DCxCombOp.fork, HandshakeOp.fork]
+theorem fork_hs_dc_equiv_fst (x : DCOp.TokenStream):
+    (DCOp.fork (x)).fst ~ (HandshakeOp.fork (x)).fst := by
+  simp [Bisim, DCOp.fork, HandshakeOp.fork]
   exists Eq
   and_intros
   · rw [corec₂_eq_tok]
     rfl
   · apply EqIsBisim
 
-theorem fork_hs_dc_equiv_snd (x : DCxCombOp.TokenStream):
-    (DCxCombOp.fork (x)).snd ~ (HandshakeOp.fork (x)).snd := by
-  simp [Bisim, DCxCombOp.fork, HandshakeOp.fork]
+theorem fork_hs_dc_equiv_snd (x : DCOp.TokenStream):
+    (DCOp.fork (x)).snd ~ (HandshakeOp.fork (x)).snd := by
+  simp [Bisim, DCOp.fork, HandshakeOp.fork]
   exists Eq
   and_intros
   · rw [corec₂_eq_tok]
@@ -76,7 +76,7 @@ def DCxCombFork := [DCxComb_com| {
     %pack1 = "DCxComb.pack" (%unpack1, %fork1) : (!ValueStream_8, !TokenStream) -> (!ValueStream_8)
     %pack2 = "DCxComb.pack" (%unpack1, %fork2) : (!ValueStream_8, !TokenStream) -> (!ValueStream_8)
     %pack12 = "DCxComb.pair" (%pack1, %pack2) : (!ValueStream_8, !ValueStream_8) -> (!ValueStream2_8)
-    "return" (%pack12) : (!ValueStream2_8) -> ()
+    "return" (%pack1, %pack2) : (!ValueStream_8, !ValueStream_8) -> ()
   }]
 /- step 2: denote dc circuit -/
 
@@ -89,9 +89,9 @@ def DCxCombFork := [DCxComb_com| {
 def ofList (vals : List (Option α)) : Stream α :=
   fun i => (vals.get? i).join
 
-def x : DCxCombOp.ValueStream (BitVec 8) := ofList [some 1, none, some 2, some 5, none]
+def x : DCOp.ValueStream (BitVec 8) := ofList [some 1, none, some 2, some 5, none]
 
-def test : CIRCTStream.DCxCombOp.ValueStream (BitVec 8) × CIRCTStream.DCxCombOp.ValueStream (BitVec 8)  :=
+def test : CIRCTStream.DCOp.ValueStream (BitVec 8) × CIRCTStream.DCOp.ValueStream (BitVec 8)  :=
   DCxCombFork.denote (Ctxt.Valuation.ofHVector (.cons x <| .nil))
 
 /- step 3: prove equivalence -/
@@ -120,7 +120,7 @@ theorem tail_iterate' {α} {n} {s : Stream' α} : Stream'.iterate Stream'.tail s
   tail_iterate''
 
 open Ctxt in
-theorem equiv_fork_fst (streamInt : DCxCombOp.ValueStream (BitVec 8)) :
+theorem equiv_fork_fst (streamInt : DCOp.ValueStream (BitVec 8)) :
   (HandshakeOp.fork streamInt).fst ~ (DCxCombFork.denote (Valuation.ofHVector (.cons streamInt <| .nil))).fst := by
   simp [EffectKind.toMonad_impure, DCxCombFork,
     EffectKind.pure_sup_pure_eq, DerivedCtxt.ofCtxt, DerivedCtxt.snoc.eq_1, get?.eq_1,
@@ -128,7 +128,7 @@ theorem equiv_fork_fst (streamInt : DCxCombOp.ValueStream (BitVec 8)) :
     Ctxt.ofList.eq_1, Com.denote_var, EffectKind.toMonad_pure, Com.denote_ret, Id.pure_eq,
     Id.bind_eq]
   sorry
-  -- unfold HandshakeOp.fork DCxCombOp.pack DCxCombOp.unpack DCxCombOp.fork
+  -- unfold HandshakeOp.fork DCOp.pack DCOp.unpack DCOp.fork
   -- simp_peephole
   -- unfold Bisim; exists Eq
   -- rw [corec₂_corec1]
@@ -206,10 +206,10 @@ def IsBisim' (R' : Stream α → Stream α → Prop) : Prop :=
     ∧ (∀ i < n, a.get i = none)
     ∧ (∀ j < m, b.get j = none)
 
-theorem corec₂_eq_corec_of_corec₂ (streamInt: DCxCombOp.ValueStream (BitVec w)) :
+theorem corec₂_eq_corec_of_corec₂ (streamInt: DCOp.ValueStream (BitVec w)) :
     (corec₂ streamInt fun x => (x 0, x 0, x.tail)).1 ≈
     corec
-      ((corec₂ streamInt fun (x : DCxCombOp.ValueStream (BitVec w)) =>
+      ((corec₂ streamInt fun (x : DCOp.ValueStream (BitVec w)) =>
             (match x 0 with
               | some val => (x 0, some (), x.tail)
               | none => (none, none, x.tail))).1,
